# Assignment 1020

## Problem 1

1. T

2. T

3. 否定。考虑表达式 $e= e_1 - e_2 = 2^{63}-1$.  constant_fold($e$)=$[[2^{63}-1]]=\{(s,2^{63}-1)\mid s\in state\}$.

   而 $[[e]]=[[e_1-e_2]]=\{\left(s, n_1-n_2\right) \mid\left(s, n_1\right) \in [[e_1 ]],\left(s, n_2\right) \in [[ e_2 ]],-2^{63} \leq n_1-n_2 \leq 2^{63}-1\}$。 由于 $[[e_1]]=[[2^{63}]]=\empty$, 所以$[[e]]=\empty$, 从而 constant_fold($e$) 与 $e$ 不语义等价

4. 不能做编译优化，因为其改变了语义！

## Problem 2

**定义**:

$\epsilon$: 空字符串

$len(l)$：字符串的长度

$l_1,l_2$: 表示将两个字符串拼接在一起

* $[[ n ]]=\{(s,\epsilon, n) \mid s \in \text { state },l\in (Z_{64})^*\}  \text{ 如果}-2^{63} \leq n \leq 2^{63}-1  $
* $[[ n ]]=\empty$  $\text{ 如果不满足}-2^{63} \leq n \leq 2^{63}-1  $
* $[[ x ]]=\{(s, \epsilon,s(x)) \mid s \in \text { state }\} $
* $[[ read\_int () ]]=\{ (s, l, l[0] \mid s \in $ state, $l \in(Z_{2^{64}})^*, len(l)= 1\}$, $l[0]$ 表示 $l$ 中的第一个数
* $[[ e_1+e_2 ]]=\left\{\left(s,(l_1,l_2), n_1+n_2\right) \mid\left(s, l_1,n_1\right) \in [[ e_1 ]],\left(s, l_2,n_2\right) \in [[ e_2 ]],-2^{63} \leq n_1+n_2 \leq 2^{63}-1,l_1 \in(Z_{2^{64}})^*,l_2 \in(Z_{2^{64}})^*\right\}$
* $[[ e_1-e_2 ]]=\left\{\left(s,(l_1,l_2), n_1-n_2\right) \mid\left(s,l_1, n_1\right) \in [[ e_1 ]],\left(s,l_2, n_2\right) \in [[ e_2 ]],-2^{63} \leq n_1-n_2 \leq 2^{63}-1, l_1 \in(Z_{2^{64}})^*,l_2 \in(Z_{2^{64}})^*\right\}$
* $[[ e_1*e_2 ]]=\left\{\left(s,(l_1,l_2), n_1*n_2\right) \mid\left(s,l_1, n_1\right) \in [[ e_1 ]],\left(s,l_2, n_2\right) \in [[ e_2 ]],-2^{63} \leq n_1*n_2 \leq 2^{63}-1,l_1 \in(Z_{2^{64}})^*,l_2 \in(Z_{2^{64}})^*\right\}$

   